coq/Soundness.v
@@ -20,11 +20,11 @@ Proof.
 Admitted.
 
 Lemma soundness :
-  forall (mdl : llvm_module) (d : llvm_definition) (s : sym_state) (m : smt_model),
+  forall (mdl : llvm_module) (fid : function_id) (s : sym_state) (m : smt_model),
     exists init_s,
-      (init_sym_state mdl d) = Some init_s ->
+      (init_sym_state mdl fid) = Some init_s ->
       multi_sym_step init_s s ->
       sat_sym_state m s ->
-      (exists init_c c, (init_state mdl d) = Some init_c /\ (multi_step c c) /\ over_approx_via s c m).
+      (exists init_c c, (init_state mdl fid) = Some init_c /\ (multi_step c c) /\ over_approx_via s c m).
 Proof.
 Admitted.
